lib/falcon/normalization_lemmas.i.dfy
@@ -1,4 +1,5 @@
 include "bv32_falcon_lemmas.i.dfy"
+include "mq_arith_lemmas.dfy"
 include "../bv16_ops.dfy"
 
 module normalization_lemmas {
@@ -7,21 +8,101 @@ module normalization_lemmas {
     import opened rv_machine
     import opened integers
     import opened ntt_512_params
+    import opened bv32_ops
+    import opened mq_arith_lemmas
 
     import bv16_ops
 
-    predicate {:opaque} buff_normlized(a: seq<uint16>)
-        ensures buff_is_nsized(a) ==> |a| == N.full;
+    const Q_HLAF :int := Q/2
+
+    // const NORMaLIZED_HIGHER_INCLUSIVE :int := Q_HLAF
+    // const NORMaLIZED_LOWER_INCLUSIVE :int := -Q_HLAF
+
+    predicate int_is_normalized(e: int)
     {
-        && (|a| == N.full)
-        && (forall i | 0 <= i < N.full :: bv16_ops.to_int16(a[i]) < Q)
+        -Q_HLAF <= e <= Q_HLAF
     }
 
-    predicate normlized_iter_inv(heap: heap_t, iter: b16_iter, address: int, index: int)
+    type nelem = e: int | int_is_normalized(e)
+
+    function normalize(e: elem): nelem
+    {
+        if e <= Q_HLAF then e else e as int - Q
+    }
+
+    function denormalize(e: nelem): elem
+    {
+        if e >= 0 then e else e + Q
+    }
+
+    predicate uint16_is_normalized(e: uint16)
+    {
+        int_is_normalized(bv16_ops.to_int16(e))
+    }
+
+    // bascially convert to int16, but with requires
+    // DOES NOT normalize a value
+    // ONLY interprets an uint16 as a normalized value
+    function uint16_as_nelem(e: uint16): nelem
+        requires uint16_is_normalized(e)
+    {
+        bv16_ops.to_int16(e)
+    }
+
+    predicate {:opaque} normalized_values(a: seq<uint16>)
+    {
+        forall i | 0 <= i < |a| :: uint16_is_normalized(a[i])
+    }
+
+    function uint16_buff_as_nelems(a: seq<uint16>): (na: seq<nelem>)
+        requires normalized_values(a);
+    {
+        reveal normalized_values();
+        seq(|a|, i requires 0 <= i < |a| => uint16_as_nelem(a[i]))
+    }
+
+    predicate normalized_iter_inv(heap: heap_t, iter: b16_iter, address: int, index: int)
     {
         && b16_iter_inv(iter, heap, if address >= 0 then address else iter.cur_ptr())
         && (index >= 0 ==> iter.index == index)
         && |iter.buff| == N.full
-        && buff_normlized(iter.buff)
+        && normalized_values(iter.buff)
+    }
+
+    lemma denormalize_lemma(buff: seq<uint16>, i: nat, a1: uint32, b: uint32, c: uint32, d: uint32)
+        requires normalized_values(buff);
+        requires i < |buff|;
+        requires a1 == uint16_sign_ext(buff[i]);
+        requires b == to_uint32(int32_rs(to_int32(a1), 31));
+        requires c == uint32_and(b, Q);
+        requires d == uint32_add(a1, c);
+        ensures uint16_is_normalized(buff[i]);
+        ensures d == denormalize(uint16_as_nelem(buff[i]));
+    {
+        assert uint16_is_normalized(buff[i]) by {
+            reveal normalized_values();
+        }
+
+        var a0 :uint16 := buff[i];
+        var sa0 := uint16_as_nelem(a0);
+        assert sa0 < 0 ==> a1 == a0 as nat + 0xffff0000;
+        assert sa0 >= 0 ==> a1 == a0;
+
+        if to_int32(a1) >= 0 {
+            assert sa0 >= 0;
+            assert b == 0 by { lemma_rs_by_31(to_int32(a1)); }
+            lemma_uint32_and_Q(b);
+            assert c == 0;
+            assert d == a0;
+            assert d == denormalize(uint16_as_nelem(a0));
+        }
+        else {
+            assert sa0 < 0;
+            assert int32_rs(to_int32(a1), 31) == -1 by { lemma_rs_by_31(to_int32(a1)); }
+            lemma_uint32_and_Q(b);
+            assert c == Q;
+            assert d == sa0 + Q;
+            assert d == denormalize(uint16_as_nelem(a0));
+        }
     }
 }
